make sealing naming consistent

heap_lang/heap.v
@@ -27,11 +27,11 @@ Definition heap_mapsto_def `{heapG Σ} (l : loc) (v: val) : iPropG heap_lang Σ 
 (* Perform sealing *)
 Module Type HeapMapstoSig.
   Parameter heap_mapsto : ∀ `{heapG Σ} (l : loc) (v: val), iPropG heap_lang Σ.
-  Axiom heap_mapsto_def : @heap_mapsto = @heap_mapsto_def.
+  Axiom heap_mapsto_eq : @heap_mapsto = @heap_mapsto_def.
 End HeapMapstoSig.
 Module Export HeapMapsto : HeapMapstoSig.
   Definition heap_mapsto := @heap_mapsto_def.
-  Definition heap_mapsto_def := Logic.eq_refl (@heap_mapsto).
+  Definition heap_mapsto_eq := Logic.eq_refl (@heap_mapsto).
 End HeapMapsto. 
 
 Definition heap_inv `{i : heapG Σ} (h : heapRA) : iPropG heap_lang Σ :=
@@ -80,8 +80,7 @@ Section heap.
     authG heap_lang Σ heapRA → nclose N ⊆ E →
     ownP σ ⊑ (|={E}=> ∃ _ : heapG Σ, heap_ctx N ∧ Π★{map σ} heap_mapsto).
   Proof.
-    rewrite heap_mapsto_def.
-    intros. rewrite -{1}(from_to_heap σ). etrans.
+    intros. rewrite heap_mapsto_eq -{1}(from_to_heap σ). etrans.
     { rewrite [ownP _]later_intro.
       apply (auth_alloc (ownP ∘ of_heap) E N (to_heap σ)); last done.
       apply to_heap_valid. }
@@ -104,8 +103,7 @@ Section heap.
   (** General properties of mapsto *)
   Lemma heap_mapsto_disjoint l v1 v2 : (l ↦ v1 ★ l ↦ v2)%I ⊑ False.
   Proof.
-    rewrite heap_mapsto_def.
-    rewrite -auto_own_op auto_own_valid map_op_singleton.
+    rewrite heap_mapsto_eq -auto_own_op auto_own_valid map_op_singleton.
     rewrite map_validI (forall_elim l) lookup_singleton.
     by rewrite option_validI excl_validI.
   Qed.
@@ -117,7 +115,7 @@ Section heap.
     P ⊑ (▷ ∀ l, l ↦ v -★ Φ (LocV l)) →
     P ⊑ || Alloc e @ E {{ Φ }}.
   Proof.
-    rewrite /heap_ctx /heap_inv heap_mapsto_def=> ?? Hctx HP.
+    rewrite /heap_ctx /heap_inv heap_mapsto_eq=> ?? Hctx HP.
     trans (|={E}=> auth_own heap_name ∅ ★ P)%I.
     { by rewrite -pvs_frame_r -(auth_empty _ E) left_id. }
     apply wp_strip_pvs, (auth_fsa heap_inv (wp_fsa (Alloc e)))
@@ -143,7 +141,7 @@ Section heap.
     P ⊑ (▷ l ↦ v ★ ▷ (l ↦ v -★ Φ v)) →
     P ⊑ || Load (Loc l) @ E {{ Φ }}.
   Proof.
-    rewrite /heap_ctx /heap_inv heap_mapsto_def=>HN ? HPΦ.
+    rewrite /heap_ctx /heap_inv heap_mapsto_eq=>HN ? HPΦ.
     apply (auth_fsa' heap_inv (wp_fsa _) id)
       with N heap_name {[ l := Excl v ]}; simpl; eauto with I.
     rewrite HPΦ{HPΦ}; apply sep_mono_r, forall_intro=> h; apply wand_intro_l.
@@ -161,7 +159,7 @@ Section heap.
     P ⊑ (▷ l ↦ v' ★ ▷ (l ↦ v -★ Φ (LitV LitUnit))) →
     P ⊑ || Store (Loc l) e @ E {{ Φ }}.
   Proof.
-    rewrite /heap_ctx /heap_inv heap_mapsto_def=>? HN ? HPΦ.
+    rewrite /heap_ctx /heap_inv heap_mapsto_eq=>? HN ? HPΦ.
     apply (auth_fsa' heap_inv (wp_fsa _) (alter (λ _, Excl v) l))
       with N heap_name {[ l := Excl v' ]}; simpl; eauto with I.
     rewrite HPΦ{HPΦ}; apply sep_mono_r, forall_intro=> h; apply wand_intro_l.
@@ -181,7 +179,7 @@ Section heap.
     P ⊑ (▷ l ↦ v' ★ ▷ (l ↦ v' -★ Φ (LitV (LitBool false)))) →
     P ⊑ || Cas (Loc l) e1 e2 @ E {{ Φ }}.
   Proof.
-    rewrite /heap_ctx /heap_inv heap_mapsto_def=>??? HN ? HPΦ.
+    rewrite /heap_ctx /heap_inv heap_mapsto_eq=>??? HN ? HPΦ.
     apply (auth_fsa' heap_inv (wp_fsa _) id)
       with N heap_name {[ l := Excl v' ]}; simpl; eauto 10 with I.
     rewrite HPΦ{HPΦ}; apply sep_mono_r, forall_intro=> h; apply wand_intro_l.
@@ -200,7 +198,7 @@ Section heap.
     P ⊑ (▷ l ↦ v1 ★ ▷ (l ↦ v2 -★ Φ (LitV (LitBool true)))) →
     P ⊑ || Cas (Loc l) e1 e2 @ E {{ Φ }}.
   Proof.
-    rewrite /heap_ctx /heap_inv heap_mapsto_def=> ?? HN ? HPΦ.
+    rewrite /heap_ctx /heap_inv heap_mapsto_eq=> ?? HN ? HPΦ.
     apply (auth_fsa' heap_inv (wp_fsa _) (alter (λ _, Excl v2) l))
       with N heap_name {[ l := Excl v1 ]}; simpl; eauto 10 with I.
     rewrite HPΦ{HPΦ}; apply sep_mono_r, forall_intro=> h; apply wand_intro_l.
